imp/ImpProofs.v
@@ -30,35 +30,35 @@ Section PROOFS.
         ge le0 v
     :
       interp_imp ge le0 (denote_expr (Var v)) =
-      interp_imp ge le0 (trigger (GetVar v)).
+      interp_imp ge le0 (u <- trigger (GetVar v);; assume (wf_val u);; Ret u).
   Proof. reflexivity. Qed.
 
   Lemma denote_expr_Lit
         ge le0 n
     :
       interp_imp ge le0 (denote_expr (Lit n)) =
-      interp_imp ge le0 (Ret n).
+      interp_imp ge le0 (assume (wf_val n);; Ret n).
   Proof. reflexivity. Qed.
 
   Lemma denote_expr_Plus
         ge le0 a b
     :
       interp_imp ge le0 (denote_expr (Plus a b)) =
-      interp_imp ge le0 (l <- denote_expr a ;; r <- denote_expr b ;; (vadd l r)?).
+      interp_imp ge le0 (l <- denote_expr a;; r <- denote_expr b;; u <- unwrapU (vadd l r);; assume (wf_val u);; Ret u).
   Proof. reflexivity. Qed.
 
   Lemma denote_expr_Minus
         ge le0 a b
     :
       interp_imp ge le0 (denote_expr (Minus a b)) =
-      interp_imp ge le0 (l <- denote_expr a ;; r <- denote_expr b ;; (vsub l r)?).
+      interp_imp ge le0 (l <- denote_expr a;; r <- denote_expr b;; u <- unwrapU (vsub l r);; assume (wf_val u);; Ret u).
   Proof. reflexivity. Qed.
 
   Lemma denote_expr_Mult
         ge le0 a b
     :
       interp_imp ge le0 (denote_expr (Mult a b)) =
-      interp_imp ge le0 (l <- denote_expr a ;; r <- denote_expr b ;; (vmul l r)?).
+      interp_imp ge le0 (l <- denote_expr a;; r <- denote_expr b;; u <- unwrapU (vmul l r);; assume (wf_val u);; Ret u).
   Proof. reflexivity. Qed.
 
   (* stmt *)
@@ -379,22 +379,33 @@ Section PROOFS.
     rewrite interp_trigger. grind.
   Qed.
 
+  Lemma interp_imp_assume_wf_val
+        ge le0 x
+    :
+      interp_imp ge le0 (assume (wf_val x);; Ret x) = assume (wf_val x);; tau;; tau;; Ret (le0, x).
+  Proof.
+    unfold interp_imp, interp_GlobEnv, interp_ImpState. grind.
+    unfold assume. grind. rewrite interp_trigger. grind.
+    unfold pure_state. grind.
+  Qed.
+
   Lemma interp_imp_expr_Var
         ge le0 v
     :
       interp_imp ge le0 (denote_expr (Var v)) =
-      r <- unwrapU (alist_find v le0);; tau;; tau;; Ret (le0, r).
+      r <- unwrapU (alist_find v le0);; tau;; tau;; assume (wf_val r);; tau;; tau;; Ret (le0, r).
   Proof.
-    apply interp_imp_GetVar.
+    rewrite denote_expr_Var. rewrite interp_imp_bind. rewrite interp_imp_GetVar.
+    grind. apply interp_imp_assume_wf_val.
   Qed.
 
   Lemma interp_imp_expr_Lit
         ge le0 n
     :
       interp_imp ge le0 (denote_expr (Lit n)) =
-      Ret (le0, n).
+      assume (wf_val n);; tau;; tau;; Ret (le0, n).
   Proof.
-    rewrite denote_expr_Lit. apply interp_imp_Ret.
+    rewrite denote_expr_Lit. apply interp_imp_assume_wf_val.
   Qed.
 
   Lemma interp_imp_expr_Plus
@@ -404,12 +415,14 @@ Section PROOFS.
       '(le1, l) <- interp_imp ge le0 (denote_expr a) ;;
       '(le2, r) <- interp_imp ge le1 (denote_expr b) ;;
       v <- (vadd l r)? ;;
+      assume (wf_val v);; tau;; tau;;
       Ret (le2, v)
   .
   Proof.
     rewrite denote_expr_Plus. rewrite interp_imp_bind.
     grind. rewrite interp_imp_bind. grind.
-    apply interp_imp_unwrapU.
+    rewrite interp_imp_bind. rewrite interp_imp_unwrapU. grind.
+    apply interp_imp_assume_wf_val.
   Qed.
 
   Lemma interp_imp_expr_Minus
@@ -419,12 +432,14 @@ Section PROOFS.
       '(le1, l) <- interp_imp ge le0 (denote_expr a) ;;
       '(le2, r) <- interp_imp ge le1 (denote_expr b) ;;
       v <- (vsub l r)? ;;
+      assume (wf_val v);; tau;; tau;;
       Ret (le2, v)
   .
   Proof.
     rewrite denote_expr_Minus. rewrite interp_imp_bind.
     grind. rewrite interp_imp_bind. grind.
-    apply interp_imp_unwrapU.
+    rewrite interp_imp_bind. rewrite interp_imp_unwrapU. grind.
+    apply interp_imp_assume_wf_val.
   Qed.
 
   Lemma interp_imp_expr_Mult
@@ -434,12 +449,14 @@ Section PROOFS.
       '(le1, l) <- interp_imp ge le0 (denote_expr a) ;;
       '(le2, r) <- interp_imp ge le1 (denote_expr b) ;;
       v <- (vmul l r)? ;;
+      assume (wf_val v);; tau;; tau;;
       Ret (le2, v)
   .
   Proof.
     rewrite denote_expr_Mult. rewrite interp_imp_bind.
     grind. rewrite interp_imp_bind. grind.
-    apply interp_imp_unwrapU.
+    rewrite interp_imp_bind. rewrite interp_imp_unwrapU. grind.
+    apply interp_imp_assume_wf_val.
   Qed.
 
   Lemma interp_imp_Assign
